Progress with Erel -> Vrel contradictions

src/FrameStack/CIU.v
@@ -208,6 +208,14 @@ Proof.
   - simpl in IHl. rewrite Heqo0 in IHl. congruence.
 Qed.
 
+Corollary match_pattern_list_tuple_vars_map :
+  forall l (f : Val -> Val), match_pattern_list [PTuple (repeat PVar (length l))] [VTuple (map f l)] = Some (map f l).
+Proof.
+  intros.
+  pose proof (match_pattern_list_tuple_vars (map f l)). rewrite map_length in H.
+  assumption.
+Qed.
+
 Lemma match_pattern_list_tuple_vars_length :
   forall m l0 vs, match_pattern_list [PTuple (repeat PVar m)] [VTuple l0] = Some vs ->
   m = length l0 /\ vs = l0.
@@ -244,6 +252,14 @@ Proof.
   - destruct a. inv Heqp. simpl in IHl. break_match_hyp. 2: congruence.
     inv Heqo. inv IHl. reflexivity.
   - destruct a. inv Heqp. simpl in IHl. break_match_hyp; congruence.
+Qed.
+
+Lemma match_pattern_list_map_vars_map :
+  forall l (f : Val*Val -> Val*Val), match_pattern_list [PMap (repeat (PVar , PVar) (length l))] [VMap (map f l)] = Some (flatten_list (map f l)).
+Proof.
+  intros.
+  pose proof (match_pattern_list_map_vars (map f l)). rewrite map_length in H.
+  assumption.
 Qed.
 
 
@@ -353,7 +369,7 @@ Proof.
   induction n; intros; cbn; auto; now rewrite IHn.
 Qed.
 
-Lemma Erel_Val_compat_closed_reverse :
+Lemma CIU_Val_compat_closed_reverse :
   forall (v v' : Val), CIU (`v) (`v') -> forall m, Vrel m v v'.
 Proof.
   valinduction; try destruct v'; intros; auto; destruct H as [Hcl1 [Hcl2 H]].
@@ -816,7 +832,10 @@ Proof.
       eexists. destruct_scopes. repeat econstructor; eauto. congruence.
     }
     (* closure - closure -> induction on m *)
-  * inv Hcl1. inv Hcl2. assert (params = params0). {
+  * inv Hcl1. inv Hcl2.
+
+    (* First, we show that the closures have the same arity with erlang:fun_info *)
+    assert (params = params0). {
       epose proof (H [FParams (ICall "erlang" "fun_info") [] [`VLit "arity"%string];FCase1 [([PLit (Z.of_nat params)], `ttrue, `VNil);([PVar], `ttrue, °inf)]] ltac:(scope_solver) _) as H0; repeat deriv.
       simpl in H11. repeat deriv. all: inv H12.
       3: inv H11.
@@ -830,8 +849,9 @@ Proof.
         simpl. rewrite Z.eqb_refl. reflexivity.
         simpl. rewrite Z.eqb_refl. reflexivity.
     }
+
+    (* Next we show that the identifiers are also equal using erlang:== *)
     assert (id = id0). {
-      (* use id comparison on closures! *)
       inv H1. inv H2.
       epose proof (H [FParams (ICall "erlang" "==") [] [` VClos ext id params0 e];FCase1 [([PLit "true"%string], `ttrue, `VNil);([PVar], `ttrue, °inf)]] ltac:(scope_solver) _) as H0; repeat deriv.
       cbn in H11.
@@ -844,128 +864,39 @@ Proof.
       destruct_scopes.
       repeat econstructor; auto. cbn.
       rewrite Nat.eqb_refl. repeat econstructor.
-    } subst. inv H1. inv H2.
-    (* apply Vrel_Clos_compat_closed; auto.
-    1-2: admit.
-    intros.
-    assert (length ext = length ext0). {
-      admit.
     }
-    assert (Erel_open (length ext + params0) e e0). {
-      admit.
-    }
-    apply H5. replace (Datatypes.length ext + params0) with
-                      (length (convert_to_closlist ext ++ vl) + 0).
-    2: {
-      simpl_convert_length. lia.
-    }
-    apply Grel_list; auto. apply biforall_app; auto.
-    eapply forall_biforall. now simpl_convert_length.
-    intros. *)
-    
-    
-    (*
-    TODO: check whether first deconstructing Vrel helps. Then 
-          apply CIU_iff_Rrel in H with a big enough index
-    
-    *)
-    
-    
-    
-    
-    generalize dependent id0. revert e0 e ext ext0 params0.
-    induction m; intros.
-    {
-      rewrite Vrel_Fix_eq. split. 2: split. 1-2: auto.
-      intuition. lia.
-    }
-    (* revert ext ext0 id0 params0 e e0 H H1 H2. induction m; intros; inv H1; inv H2.
-    - rewrite Vrel_Fix_eq. simpl. intuition; auto. lia.
-    -  *)
+
+      (* Starting the proof of Vrel clos1 clos2: *)
+      subst. inv H1. inv H2.
+
       rewrite Vrel_Fix_eq. simpl. intuition; auto.
-      (* apply Rrel_exp_compat_closed_reverse.
-      apply CIU_iff_Rrel_closed.
-      Print CIU_open. *)
-      (* TODO: instead of this, prove this with CIU_open to avoid
-         tangling up in indices *)
       (* scopes *)
       split. 2: split.
-      (* 1-2: constructor. *)
       1-2: destruct_scopes; apply -> subst_preserves_scope_exp; eauto.
       1-2: apply scoped_list_subscoped_eq; try simpl_convert_length; auto.
       2: apply biforall_length in H1; auto.
       1-2: apply Forall_app; split.
       1,3: apply closlist_scope; auto.
       1-2: apply biforall_vrel_closed in H1; apply H1.
-      
-      
-(*       intros.
-      revert m1 Hmn0 F1 F2 H2 H5.
-      assert (EXPCLOSED e.[list_subst (convert_to_closlist ext ++ vl1) idsubst]). {
-        admit.
-      }
-      assert (EXPCLOSED e0.[list_subst (convert_to_closlist ext0 ++ vl2) idsubst]). {
-        admit.
-      }
-      revert H2 H5. intros. eapply IHm. *)
-      
-      
-      
-      (* TODO: try to prove Rel_create_result with CIU! - probably won't work *)
-(*       apply CIU_iff_Rrel.
-      
-      fold (Erel m0 (e.[list_subst (convert_to_closlist ext ++ vl1) idsubst])
-                    (e0.[list_subst (convert_to_closlist ext0 ++ vl2) idsubst])). *)
-      
-      
 
-      (* evaluation *)
-      (* assert (length ext = length ext0). {
-        admit. (* try applying the last function in ext (don't use
-        induction) *)
-      } *)
-      (* assert (Erel_open (length ext + params0) e e0). {
-        apply Rrel_exp_compat_reverse. apply CIU_iff_Rrel.
-        intros ξ Hξ. split. 2: split.
-        1-2: admit.
+      (* We fold back the CIU equivalence, with value lists: *)
+      assert (H2 : CIU (RValSeq [VClos ext id0 params0 e]) (RValSeq [VClos ext0 id0 params0 e0])). {
+        split. 2: split. all: auto.
         intros.
-      }
-      intros.
-      eapply H5 in H7. all: try eassumption.
-      replace (Datatypes.length ext + params0) with
-              (length (convert_to_closlist ext ++ vl1) + 0).
-      2: {
-        simpl_convert_length. lia.
-      }
-      apply Grel_list; auto. apply biforall_app; auto.
-      eapply forall_biforall with (d1 := VNil) (d2 := VNil). now simpl_convert_length.
-      intros.
-      clear -IHm H2 Hmn0 Hmn H10.
-      (* nth i ... is a closure, next apply IHm *)
-      
-      
-      
-      
-      
-      
-      Search Erel subst. *)
-      assert (CIU (` VClos ext id0 params0 e) (` VClos ext0 id0 params0 e0)). {
-        split. 2: split. all: auto.
-      }
-      assert (H2' : CIU (RValSeq [VClos ext id0 params0 e]) (RValSeq [VClos ext0 id0 params0 e0])). {
-        split. 2: split. all: auto.
-        intros. destruct H2 as [_ [_ Hrel]].
         assert (| F, ` VClos ext id0 params0 e | ↓). {
-          inv H6. eexists. econstructor. auto. eassumption.
+          inv H5. eexists. econstructor. auto. eassumption.
         }
-        eapply Hrel in H2; auto. inv H2. inv H7. eexists. eassumption.
+        eapply H in H2; auto. inv H2. inv H7. eexists. eassumption.
         inv H0.
       }
       intros.
-      eapply CIU_iff_Rrel_closed in H2' as [_ [_ H2']].
+
+      (* We turn CIU into Rrel so that we can use equivalent frame stacks
+         instead of equal ones. *)
+      eapply CIU_iff_Rrel_closed in H2 as [_ [_ H2]].
       Unshelve. 2: exact (5 + 2 * Datatypes.length vl1 + 1 + m).
-      (* IDEA: use try to even out the evaluation counter for exceptions
-          and correct application (see repeat VNil) *)
+      (* IDEA: we use `try` to even out the evaluation counter for exceptions
+          and correct application *)
       assert (Heval_e : | FTry 1 (° EApp (` VVar 0) (map VVal vl1)) 0 (° ETuple (map VVal vl1)) :: F1,
      ` VClos ext id0 params0 e | 5 + 2 * length vl1 + 1 + m1 ↓). {
         simpl. econstructor; auto. constructor; auto. simpl.
@@ -990,6 +921,8 @@ Proof.
           assumption.
       }
 
+      (* We assert that the frame stack with the `try` expressions are equivalent
+        in as many steps that are needed to evaluate the closures. *)
       assert (Hrel : Frel (4 + 2 * length vl1 + 1 + m1) (* dirty trick here with 0 *)
           (FTry 1 (EApp (`VVar 0) (map VVal vl1)) 0 (ETuple (map VVal vl1))::F1)
           (FTry 1 (EApp (`VVar 0) (map VVal vl2)) 0 (ETuple (map VVal vl2))::F2)
@@ -1140,12 +1073,16 @@ Proof.
           specialize (H12 _ _ _ _ eq_refl). contradiction.
         * inv H7.
       }
-      
+
+      (* Finally, we combine the previous assertions with the closures
+         being in Rrel (H2). *)
       inv Heval_e.
-      epose proof (H2' := H2' _ _ _ _ Hrel H11).
+      epose proof (H2 := H2 _ _ _ _ Hrel H11).
       Unshelve. 2: lia.
-      clear -H2' H1. (* DANGER *)
-      inv H2'. deriv. simpl in H9. deriv. deriv. simpl in H3.
+      clear -H2 H1. (* DANGER, nothing else is needed for now, however this
+                               is fragile if refactoring is needed *)
+      (* We deconstruct the evaluation in the premise: *)
+      inv H2. deriv. simpl in H9. deriv. deriv. simpl in H3.
       deriv.
       rewrite map_map in H6.
       replace (map (fun x : Val => (` x).[VClos ext0 id0 (Datatypes.length vl1) e0/]) vl2) with
@@ -1168,6 +1105,844 @@ Proof.
         simpl in H4. rewrite Nat.eqb_refl in H4. eexists. eassumption.
 Qed.
 
+Definition default_subst v : Substitution := fun _ => inl v. (* Γ v := list_subst (repeat v Γ) idsubst. *)
+
+Corollary default_subst_scope Γ v :
+  VALCLOSED v ->
+  SUBSCOPE Γ ⊢ default_subst v ∷ 0.
+Proof.
+  intro.
+  unfold default_subst, subscoped. now intros.
+Qed.
+
+#[global]
+Hint Resolve default_subst_scope : core.
+
+Corollary default_subst_Grel :
+  forall m Γ v, VALCLOSED v -> Grel m Γ (default_subst v) (default_subst v).
+Proof.
+  intros. unfold Grel. split. 2: split. 1-2: auto.
+  intros. unfold default_subst.
+  now apply Vrel_Fundamental_closed.
+Qed.
+
+Ltac inf_congr :=
+  match goal with
+  | [H :  | _ , RExp (EExp inf) | _ ↓ |- _ ] => apply inf_diverges in H; contradiction
+  | [H :  | _ , RExp (EExp inf.[_]ₑ) | _ ↓ |- _ ] => apply inf_diverges in H; contradiction
+  end.
+
+Lemma inf_scope :
+  forall Γ, NVAL Γ ⊢ inf.
+Proof.
+  intros. unfold inf. scope_solver.
+Qed.
+
+#[global]
+Hint Resolve inf_scope : core.
+
+Opaque inf.
+
+Lemma redex_val_scope :
+  forall Γ (v : Val), RED Γ ⊢ `v -> VAL Γ ⊢ v.
+Proof.
+  intros. now destruct_scopes.
+Qed.
+
+Lemma ERel_Val_compat_closed_reverse :
+  forall (v v' : Val) Γ, Erel_open Γ (`v) (`v') -> Vrel_open Γ v v'.
+Proof.
+  valinduction; try destruct v'; intros; auto; intro m; intros;
+  apply Rrel_exp_compat, CIU_iff_Rrel in H as Hcontra;
+  epose proof (Hcontra_for_vars := Hcontra);
+  specialize (Hcontra (default_subst VNil) ltac:(auto)) as [_ [_ Hcontra]].
+
+  (* VNil-Var/FunId combination needs special care: *)
+  5-6: clear Hcontra; specialize (Hcontra_for_vars (default_subst (VCons VNil VNil)) ltac:(auto)) as [_ [_ Hcontra]].
+
+  1-7: epose proof (Hcontra [FCase1 [([PNil], `ttrue, `VNil);([PVar], `ttrue , °inf)]] ltac:(scope_solver) _) as Hcontra;
+       do 6 (deriv; simpl in *; try congruence); try inf_congr;
+       destruct n; congruence.
+  1,3-8: epose proof (Hcontra [FCase1 [([PLit l], `ttrue, `VNil);([PVar], `ttrue , °inf)]] ltac:(scope_solver) _) as Hcontra;
+       do 6 (deriv; simpl in *; try congruence); try inf_congr;
+       destruct n; congruence.
+  2-3,5-9: epose proof (Hcontra [FCase1 [([PCons PVar PVar], `ttrue, `VNil);([PVar], `ttrue , °inf)]] ltac:(scope_solver) _) as Hcontra;
+       do 6 (deriv; simpl in *; try congruence); try inf_congr;
+       destruct n; congruence.
+  3-5,7-10: epose proof (Hcontra [FCase1 [([PTuple (repeat PVar (length l))], `ttrue, `VNil);([PVar], `ttrue , °inf)]] ltac:(scope_solver) _) as Hcontra;
+       do 6 (deriv; simpl in *; try congruence); try inf_congr;
+       destruct n; congruence.
+  4-7,8-11: epose proof (Hcontra [FCase1 [([PMap (repeat (PVar, PVar) (length l))], `ttrue, `VNil);([PVar], `ttrue , °inf)]] ltac:(scope_solver) _) as Hcontra;
+       do 6 (deriv; simpl in *; try congruence); try inf_congr.
+  5: destruct n; congruence.
+  Unshelve. (* evaluations: *)
+    29-64:
+      apply Rrel_open_scope in H as [Hsc1 Hsc2]; apply redex_val_scope in Hsc1, Hsc2; eexists; simpl;
+      econstructor; [ auto; shelve |];
+      econstructor; [ try apply match_pattern_list_tuple_vars_map;
+                      try apply match_pattern_list_map_vars_map;
+                      simpl;
+                      try rewrite Lit_eqb_refl; try reflexivity |];
+      econstructor; [ auto; shelve |];
+      econstructor; [ try apply match_pattern_list_tuple_vars_map;
+                      try apply match_pattern_list_map_vars_map;
+                      simpl;
+                      try rewrite Lit_eqb_refl; try reflexivity |]; simpl;
+      econstructor; auto; constructor; auto.
+    Unshelve. (* scopes: *)
+      29-86: cbn; auto.
+      29-50: admit. (* technical *)
+    5, 13:
+      clear Hcontra; specialize (Hcontra_for_vars (default_subst (VCons VNil VNil)) ltac:(auto)) as [_ [_ Hcontra]];
+     epose proof (Hcontra [FCase1 [([PCons PVar PVar], `ttrue, `VNil);([PVar], `ttrue , °inf)]] ltac:(scope_solver) _) as Hcontra;
+       do 6 (deriv; simpl in *; try congruence); try inf_congr.
+    5-8,11-15: epose proof (Hcontra [FCase1 [([PNil], `ttrue, `VNil);([PVar], `ttrue , °inf)]] ltac:(scope_solver) _) as Hcontra;
+       do 6 (deriv; simpl in *; try congruence); try inf_congr.
+    Unshelve.
+     18-28: cbn. 25-28,19: destruct n.
+     18-28:
+      apply Rrel_open_scope in H as [Hsc1 Hsc2]; apply redex_val_scope in Hsc1, Hsc2; eexists; simpl;
+      econstructor; [ auto; shelve |];
+      econstructor; [ try apply match_pattern_list_tuple_vars_map;
+                      try apply match_pattern_list_map_vars_map;
+                      simpl;
+                      try rewrite Lit_eqb_refl; try reflexivity |];
+      econstructor; [ auto; shelve |];
+      econstructor; [ try apply match_pattern_list_tuple_vars_map;
+                      try apply match_pattern_list_map_vars_map;
+                      simpl;
+                      try rewrite Lit_eqb_refl; try reflexivity |]; simpl;
+      econstructor; auto; constructor; auto.
+    Unshelve.
+      18-28: cbn; auto.
+
+  * epose proof (H [FCase1 [([PLit l], `ttrue, `VNil);([PVar], `ttrue , °inf)]] ltac:(scope_solver) _) as H0; repeat deriv.
+    - simpl in H9. destruct Lit_beq eqn:EQ.
+      + apply Lit_eqb_eq in EQ. subst. choose_compat_lemma.
+      + congruence.
+    - inv H8. cbn in H11. repeat deriv. now apply inf_diverges in H11.
+    - inv H8.
+  Unshelve.
+    econstructor; econstructor; auto; econstructor;
+    [simpl; rewrite Lit_eqb_refl; reflexivity|];
+    simpl; econstructor; auto; econstructor;
+    [simpl; rewrite Lit_eqb_refl; reflexivity|]; constructor; auto;
+    constructor; auto.
+  * choose_compat_lemma.
+    - apply IHv1. destruct_scopes. split. 2: split. 1-2: auto.
+      intros. epose proof (H (FCase1 [([PCons PVar PVar], `ttrue, `VVar 0);([PVar], `ttrue , °inf)] :: F) ltac:(scope_solver) _) as H2; repeat deriv.
+      + inv H16. cbn in H17. repeat deriv. inv H16. cbn in H17. now exists k1.
+      + inv H16.
+      + inv H15.
+    - apply IHv2. destruct_scopes. split. 2: split. 1-2: auto.
+      intros. epose proof (H (FCase1 [([PCons PVar PVar], `ttrue, `VVar 1);([PVar], `ttrue , °inf)] :: F) ltac:(scope_solver) _) as H2; repeat deriv.
+      + inv H16. cbn in H17. repeat deriv. inv H16. cbn in H17. now exists k1.
+      + inv H16.
+      + inv H15.
+  Unshelve.
+    all: auto.
+    all: destruct H1; destruct_scopes; econstructor; econstructor; auto;
+       econstructor; [reflexivity|]; simpl; econstructor; auto;
+       econstructor; [reflexivity|]; eauto.
+  (* Tuple *)
+  * choose_compat_lemma.
+    revert l0 Hcl2 H. induction l; destruct l0; intros.
+    - now auto.
+    - epose proof (H [FCase1 [([PTuple []], `ttrue, `VNil);([PVar], `ttrue , °inf)]] ltac:(scope_solver) _) as H0; repeat deriv.
+      + inv H9.
+      + cbn in H11. repeat deriv. now apply inf_diverges in H12.
+      + now inv H8.
+    - epose proof (H [FCase1 [([PTuple (repeat PVar (length (a :: l)))], `ttrue, `VNil);([PVar], `ttrue , °inf)]] ltac:(scope_solver) _) as H0; repeat deriv.
+      + inv H9.
+      + cbn in H11. repeat deriv. now apply inf_diverges in H12.
+      + now inv H8.
+    - inv IHv.
+      assert (REDCLOSED (`VTuple l) /\ REDCLOSED (`VTuple l0)) as [IS1 IS2]. {
+        destruct_scopes. split; do 3 constructor; intros;
+        try apply (H4 (S i)); try apply (H5 (S i)); slia.
+      }
+      assert (forall F : FrameStack, FSCLOSED F -> | F, ` VTuple l | ↓ -> | F, ` VTuple l0 | ↓) as IS3. {
+        intros.
+        epose proof (H (FCase1 [([PTuple (repeat PVar (length (a :: l)))], `ttrue, `VTuple (varsFrom 1 (length l)));([PVar], `ttrue , °inf)] :: F) _ _) as H4.
+        repeat deriv.
+        * pose proof (match_pattern_list_tuple_vars_length (1 + length l) (v::l0) vs') as H1. simpl repeat in H1.
+          apply H1 in H14 as H14'. destruct H14' as [Hlen EQ].
+          simpl length in *. clear H1. inv EQ.
+          simpl in H15. repeat deriv.
+          rewrite H14 in H16. inv H16. simpl in H17.
+          pose proof (map_varsFrom (length l) 1 (v :: l0) ltac:(slia)) as H17'.
+          simpl in H17'. rewrite H17' in H17.
+          replace (length l) with (length l0) in H17 by lia.
+          rewrite firstn_all in H17. now exists k1.
+        * cbn in H16. repeat deriv. now apply inf_diverges in H17.
+        * inv H13.
+      }
+      specialize (IHl H3 IS1 _ IS2 IS3).
+      constructor; auto.
+      + apply H2. apply biforall_length in IHl as Hlen.
+        split. 2: split.
+        1-2: do 2 constructor; destruct_scopes; try apply (H6 0); try apply (H7 0); slia.
+        intros. epose proof (H (FCase1 [([PTuple (repeat PVar (length (a :: l)))], `ttrue, `VVar 0);([PVar], `ttrue , °inf)] :: F) ltac:(scope_solver) _) as H4; repeat deriv.
+        ** pose proof (match_pattern_list_tuple_vars (v :: l0)) as H1.
+           simpl repeat in H1. rewrite <-Hlen in H1. rewrite H1 in H14.
+           inv H14. simpl in H15. repeat deriv.
+           rewrite H1 in H15. inv H15. simpl in H16. now exists k1.
+        ** pose proof (match_pattern_list_tuple_vars (v :: l0)) as H1.
+           simpl repeat in H1. rewrite <-Hlen in H1. rewrite H1 in H14.
+           congruence.
+        ** inv H13.
+    Unshelve.
+      all: auto.
+      3: {
+        constructor; auto. constructor; intros; destruct i.
+        - do 2 constructor.
+        - cbn. destruct i. do 2 constructor. destruct i; auto.
+        - do 2 constructor; intros.
+          rewrite varsFrom_length in H5. simpl.
+          rewrite scope_repeat_var.
+          pose proof (varsFrom_scope (length l) 1 i).
+          eapply loosen_scope_val. 2: eassumption. lia.
+        - simpl in *. destruct i. 2: lia.
+          simpl. scope_solver.
+      }
+      {
+        destruct_scopes; econstructor; econstructor; auto; econstructor;
+        [reflexivity|]; simpl; econstructor; auto; econstructor;
+        [reflexivity|]; constructor; auto;
+        constructor; auto.
+      }
+      {
+        destruct_scopes; econstructor; econstructor; auto; econstructor;
+        [apply match_pattern_list_tuple_vars|]; simpl; econstructor; auto. econstructor;
+        [apply (match_pattern_list_tuple_vars (a :: l))|]; constructor; auto;
+        constructor; auto.
+      }
+      {
+        inv H1. inv H4. 2: { inv H1. }
+        destruct_scopes; econstructor; econstructor; auto; econstructor;
+        [apply match_pattern_list_tuple_vars|]; simpl; econstructor; auto. econstructor; simpl;
+        [apply (match_pattern_list_tuple_vars (a :: l))|]; constructor; auto; rewrite map_varsFrom; try slia; simpl; rewrite firstn_all; eauto.
+      }
+      {
+        inv H1. inv H4. 2: { inv H1. }
+        destruct_scopes; econstructor; econstructor; auto; econstructor;
+        [apply match_pattern_list_tuple_vars|]; simpl; econstructor; auto. econstructor; simpl;
+        [apply (match_pattern_list_tuple_vars (a :: l))|]; constructor; auto. simpl. eassumption.
+      }
+  (* Map *)
+  * choose_compat_lemma.
+    revert l0 Hcl2 H. induction l; destruct l0; intros.
+    - now auto.
+    - epose proof (H [FCase1 [([PMap []], `ttrue, `VNil);([PVar], `ttrue , °inf)]] ltac:(scope_solver) _) as H0; repeat deriv.
+      + inv H9.
+      + cbn in H11. repeat deriv. now apply inf_diverges in H12.
+      + now inv H8.
+    - epose proof (H [FCase1 [([PMap (repeat (PVar, PVar) (length (a :: l)))], `ttrue, `VNil);([PVar], `ttrue , °inf)]] ltac:(scope_solver) _) as H0; repeat deriv.
+      + inv H9.
+      + cbn in H11. repeat deriv. now apply inf_diverges in H12.
+      + now inv H8.
+    - inv IHv.
+      assert (REDCLOSED (`VMap l) /\ REDCLOSED (`VMap l0)) as [IS1 IS2]. {
+        destruct_scopes. split; do 3 constructor; intros;
+        try apply (H1 (S i)); try apply (H4 (S i));
+        try apply (H7 (S i)); try apply (H8 (S i)); try slia.
+      }
+      assert (forall F : FrameStack, FSCLOSED F -> | F, ` VMap l | ↓ -> | F, ` VMap l0 | ↓) as IS3. {
+        intros.
+        epose proof (H (FCase1 [([PMap (repeat (PVar, PVar) (length (a :: l)))], `ttrue, `VMap (deflatten_list (varsFrom 2 (length (flatten_list l)))));([PVar], `ttrue , °inf)] :: F) _ _) as H4.
+        repeat deriv.
+        * pose proof (match_pattern_list_map_vars_length (1 + length l) (p::l0) vs') as H1. simpl repeat in H1.
+          apply H1 in H14 as H14'. destruct H14' as [Hlen EQ].
+          simpl length in *. clear H1. inv EQ.
+          simpl in H15. repeat deriv.
+          rewrite H14 in H16. inv H16. simpl in H17.
+          destruct p.
+          pose proof (length_flatten_list l) as Hlen1.
+          pose proof (length_flatten_list l0) as Hlen2.
+          pose proof (map_varsFrom (length (flatten_list l)) 2 (v :: v0 :: flatten_list l0) ltac:(slia)) as H17'.
+          replace (map
+          (fun '(x, y) =>
+           (x.[list_subst (v :: v0 :: flatten_list l0) idsubst]ᵥ,
+            y.[list_subst (v :: v0 :: flatten_list l0) idsubst]ᵥ))
+          (deflatten_list (varsFrom 2 (Datatypes.length (flatten_list l))))) with
+                  (deflatten_list (map (fun x : Val => x.[list_subst (v :: v0 :: flatten_list l0) idsubst]ᵥ)
+                  (varsFrom 2 (Datatypes.length (flatten_list l))))) in H17.
+          2: {
+            replace (length (flatten_list l)) with (length (flatten_list l0)) by lia.
+            clear. rewrite deflatten_map. reflexivity.
+          }
+          simpl in H17', H17.
+          rewrite H17' in H17.
+          replace (length (flatten_list l)) with (length (flatten_list l0)) in H17 by lia.
+          rewrite firstn_all in H17.
+          rewrite flatten_deflatten in H17. now exists k1.
+        * cbn in H16. repeat deriv. now apply inf_diverges in H17.
+        * inv H13.
+      }
+      specialize (IHl H3 IS1 _ IS2 IS3). destruct a, p.
+      constructor; auto. split.
+      + apply H2. simpl. apply biforall_length in IHl as Hlen.
+        split. 2: split.
+        1-2: do 2 constructor; destruct_scopes; try apply (H5 0); try apply (H6 0); slia.
+        intros. epose proof (H (FCase1 [([PMap (repeat (PVar, PVar) (length ((v1, v2) :: l)))], `ttrue, `VVar 0);([PVar], `ttrue , °inf)] :: F) ltac:(scope_solver) _) as H4; repeat deriv.
+        ** pose proof (match_pattern_list_map_vars ((v1, v2) :: l0)) as H1.
+          simpl repeat in H1. rewrite <-Hlen in H1. rewrite H1 in H14.
+          inv H14. simpl in H15. repeat deriv.
+          rewrite H1 in H15. inv H15. simpl in H16. now exists k1.
+        ** pose proof (match_pattern_list_map_vars ((v1, v2) :: l0)) as H1.
+          simpl repeat in H1. rewrite <-Hlen in H1. rewrite H1 in H14.
+          congruence.
+        ** inv H13.
+    + apply H2. simpl. apply biforall_length in IHl as Hlen.
+      split. 2: split.
+      1-2: do 2 constructor; destruct_scopes; try apply (H11 0); try apply (H12 0); slia.
+      intros. epose proof (H (FCase1 [([PMap (repeat (PVar, PVar) (length ((v1, v2) :: l)))], `ttrue, `VVar 1);([PVar], `ttrue , °inf)] :: F) ltac:(scope_solver) _) as H4; repeat deriv.
+      ** pose proof (match_pattern_list_map_vars ((v1, v2) :: l0)) as H1.
+        simpl repeat in H1. rewrite <-Hlen in H1. rewrite H1 in H14.
+        inv H14. simpl in H15. repeat deriv.
+        rewrite H1 in H15. inv H15. simpl in H16. now exists k1.
+      ** pose proof (match_pattern_list_map_vars ((v1, v2) :: l0)) as H1.
+        simpl repeat in H1. rewrite <-Hlen in H1. rewrite H1 in H14.
+        congruence.
+      ** inv H13.
+    Unshelve.
+    all: auto.
+    3: {
+      constructor; auto. constructor; intros; destruct i.
+      - do 2 constructor.
+      - cbn. destruct i. do 2 constructor. destruct i; auto.
+      - simpl. constructor. apply VMap_scope_Forall, deflatten_keeps_prop.
+        rewrite indexed_to_forall with (def := VNil). intros.
+        rewrite length_flatten_list.
+        rewrite scope_repeat_var_prod.
+        pose proof (varsFrom_scope (length l * 2) 2 i).
+        eapply loosen_scope_val. 2: exact H6.
+        rewrite varsFrom_length, length_flatten_list in H5. lia.
+      - simpl in *. destruct i. 2: lia.
+        simpl. scope_solver.
+    }
+    {
+      destruct_scopes; econstructor; econstructor; auto; econstructor;
+      [reflexivity|]; simpl; econstructor; auto; econstructor;
+      [reflexivity|]; constructor; auto;
+      constructor; auto.
+    }
+    {
+      destruct_scopes; econstructor; econstructor; auto; econstructor;
+      [apply match_pattern_list_map_vars|]; simpl; econstructor; auto. econstructor;
+      [apply (match_pattern_list_map_vars (a :: l))|]; constructor; auto;
+      constructor; auto.
+    }
+    {
+      inv H1. inv H4. 2: { inv H1. }
+      destruct_scopes; econstructor; econstructor; auto; econstructor;
+      [apply match_pattern_list_map_vars|]; simpl; econstructor; auto. econstructor; simpl;
+      [apply (match_pattern_list_map_vars (a :: l))|].
+      rewrite deflatten_map.
+      constructor; auto.
+      * rewrite map_varsFrom.
+        2: destruct a; slia.
+        destruct a. simpl. rewrite firstn_all, flatten_deflatten.
+        constructor; intros; try apply H10; try apply H16; assumption.
+      * rewrite map_varsFrom.
+        2: destruct a; slia.
+        destruct a. simpl. rewrite firstn_all, flatten_deflatten. eassumption.
+    }
+    {
+      inv H1. inv H4. 2: { inv H1. }
+      destruct_scopes; econstructor; econstructor; auto. econstructor;      
+      [apply (match_pattern_list_map_vars ((v, v0)::l))|]; simpl; econstructor; auto. simpl. econstructor;
+      [apply (match_pattern_list_map_vars ((v, v0) :: l))|]; constructor; auto. simpl. eassumption.
+    }
+    {
+      inv H1. inv H4. 2: { inv H1. }
+      destruct_scopes; econstructor; econstructor; auto. econstructor;      
+      [apply (match_pattern_list_map_vars ((v, v0)::l))|]; simpl; econstructor; auto. simpl. econstructor;
+      [apply (match_pattern_list_map_vars ((v, v0) :: l))|]; constructor; auto. simpl. eassumption.
+    }
+  (* closures - anything : create different exceptions in a try expr.
+     e.g., apply the closure with a non-matching argument number, 
+     then match on the exception:
+      - if it's badarity -> result is VNil
+      - if it's badfun -> result is divergence
+    TODO: The following proof is identical for the next 7 cases
+  *)
+  * destruct params.
+    (* we have to make sure, that the number of parameters differ *)
+    - epose proof (H [FApp1 [`VNil];FTry 1 (`VNil) 3 (ECase (`VVar 1) [
+        ([PLit "badarity"%string], `ttrue, `VNil);
+        ([PVar], `ttrue, °inf)
+      ])] ltac:(scope_solver) _) as H0; repeat deriv.
+      cbn in H10. repeat deriv. cbn in H12.
+      2: { now specialize (H5 _ _ _ _ eq_refl). }
+      repeat deriv. inv H12. 2: inv H11. inv H11. cbn in H14.
+      repeat deriv. now apply inf_diverges in H14.
+    - epose proof (H [FApp1 [];FTry 1 (`VNil) 3 (ECase (`VVar 1) [
+        ([PLit "badarity"%string], `ttrue, `VNil);
+        ([PVar], `ttrue, °inf)
+      ])] ltac:(scope_solver) _) as H0; repeat deriv.
+      cbn in H8. repeat deriv. cbn in H11.
+      2: { now specialize (H5 _ _ _ _ eq_refl). }
+      repeat deriv. inv H11. 2: inv H10. inv H10. cbn in H13.
+      repeat deriv. now apply inf_diverges in H13.
+    Unshelve.
+    {
+      eexists. destruct_scopes. repeat econstructor; eauto. congruence.
+    }
+    {
+      eexists. destruct_scopes. repeat econstructor; eauto. congruence.
+    }
+  * destruct params.
+  (* we have to make sure, that the number of parameters differ *)
+    - epose proof (H [FApp1 [`VNil];FTry 1 (`VNil) 3 (ECase (`VVar 1) [
+        ([PLit "badarity"%string], `ttrue, `VNil);
+        ([PVar], `ttrue, °inf)
+      ])] ltac:(scope_solver) _) as H0; repeat deriv.
+      cbn in H10. repeat deriv. cbn in H12.
+      2: { now specialize (H5 _ _ _ _ eq_refl). }
+      repeat deriv. inv H12. 2: inv H11. inv H11. cbn in H14.
+      repeat deriv. now apply inf_diverges in H14.
+    - epose proof (H [FApp1 [];FTry 1 (`VNil) 3 (ECase (`VVar 1) [
+        ([PLit "badarity"%string], `ttrue, `VNil);
+        ([PVar], `ttrue, °inf)
+      ])] ltac:(scope_solver) _) as H0; repeat deriv.
+      cbn in H8. repeat deriv. cbn in H11.
+      2: { now specialize (H5 _ _ _ _ eq_refl). }
+      repeat deriv. inv H11. 2: inv H10. inv H10. cbn in H13.
+      repeat deriv. now apply inf_diverges in H13.
+    Unshelve.
+    {
+      eexists. destruct_scopes. repeat econstructor; eauto. congruence.
+    }
+    {
+      eexists. destruct_scopes. repeat econstructor; eauto. congruence.
+    }
+  * destruct params.
+  (* we have to make sure, that the number of parameters differ *)
+    - epose proof (H [FApp1 [`VNil];FTry 1 (`VNil) 3 (ECase (`VVar 1) [
+        ([PLit "badarity"%string], `ttrue, `VNil);
+        ([PVar], `ttrue, °inf)
+      ])] ltac:(scope_solver) _) as H0; repeat deriv.
+      cbn in H10. repeat deriv. cbn in H12.
+      2: { now specialize (H5 _ _ _ _ eq_refl). }
+      repeat deriv. inv H12. 2: inv H11. inv H11. cbn in H14.
+      repeat deriv. now apply inf_diverges in H14.
+    - epose proof (H [FApp1 [];FTry 1 (`VNil) 3 (ECase (`VVar 1) [
+        ([PLit "badarity"%string], `ttrue, `VNil);
+        ([PVar], `ttrue, °inf)
+      ])] ltac:(scope_solver) _) as H0; repeat deriv.
+      cbn in H8. repeat deriv. cbn in H11.
+      2: { now specialize (H5 _ _ _ _ eq_refl). }
+      repeat deriv. inv H11. 2: inv H10. inv H10. cbn in H13.
+      repeat deriv. now apply inf_diverges in H13.
+    Unshelve.
+    {
+      eexists. destruct_scopes. repeat econstructor; eauto. congruence.
+    }
+    {
+      eexists. destruct_scopes. repeat econstructor; eauto. congruence.
+    }
+  * destruct params.
+  (* we have to make sure, that the number of parameters differ *)
+    - epose proof (H [FApp1 [`VNil];FTry 1 (`VNil) 3 (ECase (`VVar 1) [
+        ([PLit "badarity"%string], `ttrue, `VNil);
+        ([PVar], `ttrue, °inf)
+      ])] ltac:(scope_solver) _) as H0; repeat deriv.
+      cbn in H10. repeat deriv. cbn in H12.
+      2: { now specialize (H5 _ _ _ _ eq_refl). }
+      repeat deriv. inv H12. 2: inv H11. inv H11. cbn in H14.
+      repeat deriv. now apply inf_diverges in H14.
+    - epose proof (H [FApp1 [];FTry 1 (`VNil) 3 (ECase (`VVar 1) [
+        ([PLit "badarity"%string], `ttrue, `VNil);
+        ([PVar], `ttrue, °inf)
+      ])] ltac:(scope_solver) _) as H0; repeat deriv.
+      cbn in H8. repeat deriv. cbn in H11.
+      2: { now specialize (H5 _ _ _ _ eq_refl). }
+      repeat deriv. inv H11. 2: inv H10. inv H10. cbn in H13.
+      repeat deriv. now apply inf_diverges in H13.
+    Unshelve.
+    {
+      eexists. destruct_scopes. repeat econstructor; eauto. congruence.
+    }
+    {
+      eexists. destruct_scopes. repeat econstructor; eauto. congruence.
+    }
+  * destruct params.
+  (* we have to make sure, that the number of parameters differ *)
+    - epose proof (H [FApp1 [`VNil];FTry 1 (`VNil) 3 (ECase (`VVar 1) [
+        ([PLit "badarity"%string], `ttrue, `VNil);
+        ([PVar], `ttrue, °inf)
+      ])] ltac:(scope_solver) _) as H0; repeat deriv.
+      cbn in H10. repeat deriv. cbn in H12.
+      2: { now specialize (H5 _ _ _ _ eq_refl). }
+      repeat deriv. inv H12. 2: inv H11. inv H11. cbn in H14.
+      repeat deriv. now apply inf_diverges in H14.
+    - epose proof (H [FApp1 [];FTry 1 (`VNil) 3 (ECase (`VVar 1) [
+        ([PLit "badarity"%string], `ttrue, `VNil);
+        ([PVar], `ttrue, °inf)
+      ])] ltac:(scope_solver) _) as H0; repeat deriv.
+      cbn in H8. repeat deriv. cbn in H11.
+      2: { now specialize (H5 _ _ _ _ eq_refl). }
+      repeat deriv. inv H11. 2: inv H10. inv H10. cbn in H13.
+      repeat deriv. now apply inf_diverges in H13.
+    Unshelve.
+    {
+      eexists. destruct_scopes. repeat econstructor; eauto. congruence.
+    }
+    {
+      eexists. destruct_scopes. repeat econstructor; eauto. congruence.
+    }
+  * destruct params.
+  (* we have to make sure, that the number of parameters differ *)
+    - epose proof (H [FApp1 [`VNil];FTry 1 (`VNil) 3 (ECase (`VVar 1) [
+        ([PLit "badarity"%string], `ttrue, `VNil);
+        ([PVar], `ttrue, °inf)
+      ])] ltac:(scope_solver) _) as H0; repeat deriv.
+      cbn in H10. repeat deriv. cbn in H12.
+      2: { now specialize (H5 _ _ _ _ eq_refl). }
+      repeat deriv. inv H12. 2: inv H11. inv H11. cbn in H14.
+      repeat deriv. now apply inf_diverges in H14.
+    - epose proof (H [FApp1 [];FTry 1 (`VNil) 3 (ECase (`VVar 1) [
+        ([PLit "badarity"%string], `ttrue, `VNil);
+        ([PVar], `ttrue, °inf)
+      ])] ltac:(scope_solver) _) as H0; repeat deriv.
+      cbn in H8. repeat deriv. cbn in H11.
+      2: { now specialize (H5 _ _ _ _ eq_refl). }
+      repeat deriv. inv H11. 2: inv H10. inv H10. cbn in H13.
+      repeat deriv. now apply inf_diverges in H13.
+    Unshelve.
+    {
+      eexists. destruct_scopes. repeat econstructor; eauto. congruence.
+    }
+    {
+      eexists. destruct_scopes. repeat econstructor; eauto. congruence.
+    }
+  * destruct params.
+  (* we have to make sure, that the number of parameters differ *)
+    - epose proof (H [FApp1 [`VNil];FTry 1 (`VNil) 3 (ECase (`VVar 1) [
+        ([PLit "badarity"%string], `ttrue, `VNil);
+        ([PVar], `ttrue, °inf)
+      ])] ltac:(scope_solver) _) as H0; repeat deriv.
+      cbn in H10. repeat deriv. cbn in H12.
+      2: { now specialize (H5 _ _ _ _ eq_refl). }
+      repeat deriv. inv H12. 2: inv H11. inv H11. cbn in H14.
+      repeat deriv. now apply inf_diverges in H14.
+    - epose proof (H [FApp1 [];FTry 1 (`VNil) 3 (ECase (`VVar 1) [
+        ([PLit "badarity"%string], `ttrue, `VNil);
+        ([PVar], `ttrue, °inf)
+      ])] ltac:(scope_solver) _) as H0; repeat deriv.
+      cbn in H8. repeat deriv. cbn in H11.
+      2: { now specialize (H5 _ _ _ _ eq_refl). }
+      repeat deriv. inv H11. 2: inv H10. inv H10. cbn in H13.
+      repeat deriv. now apply inf_diverges in H13.
+    Unshelve.
+    {
+      eexists. destruct_scopes. repeat econstructor; eauto. congruence.
+    }
+    {
+      eexists. destruct_scopes. repeat econstructor; eauto. congruence.
+    }
+    (* closure - closure -> induction on m *)
+  * inv Hcl1. inv Hcl2.
+
+    (* First, we show that the closures have the same arity with erlang:fun_info *)
+    assert (params = params0). {
+      epose proof (H [FParams (ICall "erlang" "fun_info") [] [`VLit "arity"%string];FCase1 [([PLit (Z.of_nat params)], `ttrue, `VNil);([PVar], `ttrue, °inf)]] ltac:(scope_solver) _) as H0; repeat deriv.
+      simpl in H11. repeat deriv. all: inv H12.
+      3: inv H11.
+      1-2: destruct (Z.of_nat params0 =? Z.of_nat params)%Z eqn:P; inv H5.
+      - apply Z.eqb_eq in P. now apply Znat.Nat2Z.inj in P.
+      - simpl in H14. repeat deriv. now apply inf_diverges in H14. 
+      Unshelve.
+        congruence.
+        auto.
+        destruct_scopes. repeat econstructor; auto.
+        simpl. rewrite Z.eqb_refl. reflexivity.
+        simpl. rewrite Z.eqb_refl. reflexivity.
+    }
+
+    (* Next we show that the identifiers are also equal using erlang:== *)
+    assert (id = id0). {
+      inv H1. inv H2.
+      epose proof (H [FParams (ICall "erlang" "==") [] [` VClos ext id params0 e];FCase1 [([PLit "true"%string], `ttrue, `VNil);([PVar], `ttrue, °inf)]] ltac:(scope_solver) _) as H0; repeat deriv.
+      cbn in H11.
+      break_match_hyp. now apply Nat.eqb_eq in Heqb.
+      repeat deriv; inv H12; inv H11.  simpl in *.
+      repeat deriv. now apply inf_diverges in H13.
+    Unshelve.
+      congruence.
+      auto.
+      destruct_scopes.
+      repeat econstructor; auto. cbn.
+      rewrite Nat.eqb_refl. repeat econstructor.
+    }
+
+      (* Starting the proof of Vrel clos1 clos2: *)
+      subst. inv H1. inv H2.
+
+      rewrite Vrel_Fix_eq. simpl. intuition; auto.
+      (* scopes *)
+      split. 2: split.
+      1-2: destruct_scopes; apply -> subst_preserves_scope_exp; eauto.
+      1-2: apply scoped_list_subscoped_eq; try simpl_convert_length; auto.
+      2: apply biforall_length in H1; auto.
+      1-2: apply Forall_app; split.
+      1,3: apply closlist_scope; auto.
+      1-2: apply biforall_vrel_closed in H1; apply H1.
+
+      (* We fold back the CIU equivalence, with value lists: *)
+      assert (H2 : CIU (RValSeq [VClos ext id0 params0 e]) (RValSeq [VClos ext0 id0 params0 e0])). {
+        split. 2: split. all: auto.
+        intros.
+        assert (| F, ` VClos ext id0 params0 e | ↓). {
+          inv H5. eexists. econstructor. auto. eassumption.
+        }
+        eapply H in H2; auto. inv H2. inv H7. eexists. eassumption.
+        inv H0.
+      }
+      intros.
+
+      (* We turn CIU into Rrel so that we can use equivalent frame stacks
+         instead of equal ones. *)
+      eapply CIU_iff_Rrel_closed in H2 as [_ [_ H2]].
+      Unshelve. 2: exact (5 + 2 * Datatypes.length vl1 + 1 + m).
+      (* IDEA: we use `try` to even out the evaluation counter for exceptions
+          and correct application *)
+      assert (Heval_e : | FTry 1 (° EApp (` VVar 0) (map VVal vl1)) 0 (° ETuple (map VVal vl1)) :: F1,
+     ` VClos ext id0 params0 e | 5 + 2 * length vl1 + 1 + m1 ↓). {
+        simpl. econstructor; auto. constructor; auto. simpl.
+        replace (map (fun x : Exp => x.[VClos ext id0 params0 e/]) (map VVal vl1))
+           with (map VVal vl1).
+        2: {
+          clear -H1. rewrite map_map. simpl.
+          apply biforall_vrel_closed in H1 as [H1 _].
+          apply map_ext_Forall. induction vl1; inv H1; constructor; auto.
+          now rewrite vclosed_ignores_sub.
+        }
+        do 2 constructor. auto.
+        constructor. destruct vl1.
+        * simpl. econstructor. congruence. reflexivity. simpl.
+          break_match_goal. 2: apply Nat.eqb_neq in Heqb; simpl in H0; lia.
+          assumption.
+        * simpl. constructor. congruence.
+          simpl. change clock to (S (1 + 2 * length vl1) + m1).
+          inv H1. constructor. now apply Vrel_closed_l in H9.
+          eapply step_term_term_plus. apply params_eval_create.
+          now apply biforall_vrel_closed in H11. simpl. rewrite Nat.eqb_refl.
+          assumption.
+      }
+
+      (* We assert that the frame stack with the `try` expressions are equivalent
+        in as many steps that are needed to evaluate the closures. *)
+      assert (Hrel : Frel (4 + 2 * length vl1 + 1 + m1) (* dirty trick here with 0 *)
+          (FTry 1 (EApp (`VVar 0) (map VVal vl1)) 0 (ETuple (map VVal vl1))::F1)
+          (FTry 1 (EApp (`VVar 0) (map VVal vl2)) 0 (ETuple (map VVal vl2))::F2)
+            ). {
+        clear Heval_e.
+        split. 2: split. 1-2: constructor; [constructor|apply H5].
+        1-4: do 2 constructor; auto; apply indexed_to_forall; apply biforall_vrel_closed in H1; clear -H1.
+
+        (* boiler plate codes: *)
+        1-2: destruct H1 as [H1 _]; induction vl1; simpl; auto; inv H1; constructor;
+             [ constructor; eapply loosen_scope_val; [|eassumption]; lia | auto].
+        1-2: destruct H1 as [_ H1]; induction vl2; simpl; auto; inv H1; constructor;
+             [ constructor; eapply loosen_scope_val; [|eassumption]; lia | auto].
+        (****)
+
+        split. 2: split.
+        all: intros.
+        * deriv. inv H7. inv H16. inv H8. 2: inv H16.
+          simpl in H17.
+          deriv. deriv. deriv. inv H1.
+          - deriv.
+            simpl in Hmn1.
+            pose proof (Rel_create_result _ [] [] (IApp hd) (IApp hd') ltac:(auto) ltac:(constructor; eauto)).
+            intuition.
+            + repeat destruct_hyps.
+              specialize (H1 k ltac:(lia)) as [Hrel [Eq1 Eq2]].
+              rewrite Eq1 in H14. eapply Hrel in H14 as [kk D]. 2: reflexivity.
+              2: eapply Frel_downclosed in H5; eassumption.
+              eexists. constructor; auto. simpl.
+              constructor; auto. constructor; auto. now apply Vrel_closed_r in H0.
+              constructor. econstructor. congruence. reflexivity.
+              rewrite Eq2. exact D.
+              Unshelve. lia.
+            + repeat destruct_hyps. rewrite H7 in H14.
+              eapply H5 in H14 as [kk D]. 2: lia. 2: eapply biforall_impl;[|eassumption]; intros; downclose_Vrel.
+              eexists. constructor; auto. simpl.
+              constructor; auto. constructor; auto. now apply Vrel_closed_r in H0.
+              constructor. econstructor. congruence. reflexivity.
+              rewrite H9. exact D.
+              Unshelve. lia.
+            + repeat destruct_hyps. rewrite H7 in H14.
+              eapply H5 in H14 as [kk D]. 2: lia. 2: eapply Excrel_downclosed; eassumption.
+              eexists. constructor; auto. simpl.
+              constructor; auto. constructor; auto. now apply Vrel_closed_r in H0.
+              constructor. econstructor. congruence. reflexivity.
+              rewrite H9. exact D.
+              Unshelve. lia.
+          - inv H13. inv H18.
+            rewrite map_map in H12.
+            rewrite vclosed_ignores_sub in H10. 2: now apply Vrel_closed_l in H7.
+            replace (map (fun x : Val => (` x).[hd/]) tl) with
+                    (map VVal tl) in H12.
+            2: {
+              clear -H9. simpl.
+              apply biforall_vrel_closed in H9 as [H1 _].
+              apply map_ext_Forall. induction tl; inv H1; constructor; auto.
+              now rewrite vclosed_ignores_sub.
+            }
+            rewrite vclosed_ignores_sub in H12. 2: now apply Vrel_closed_l in H0.
+            eapply term_step_term in H12. 2: apply params_eval_create.
+            2: now apply biforall_vrel_closed in H9.
+            simpl app in H12.
+            simpl in Hmn1.
+            assert (list_biforall (Vrel (k0 - (1 + 2 * Datatypes.length tl)))
+                                  (hd0 :: tl) (hd'0 :: tl') ) as Hfinally.
+            {
+              constructor. downclose_Vrel.
+              eapply biforall_impl. 2: eassumption. intros. downclose_Vrel.
+            }
+            epose proof (Rel_create_result_relaxed _ (hd0 :: tl) (hd'0 :: tl') (IApp hd) (IApp hd') Hfinally _). Unshelve.
+            4: {
+              split. 2: split.
+              1-2: constructor; now apply Vrel_closed in H0.
+              downclose_Vrel.
+            }
+            intuition.
+            + repeat destruct_hyps. simpl in Hmn1.
+              specialize (H1 (k0 - (1 + 2 * Datatypes.length tl)) ltac:(lia)).
+              destruct H1 as [Hrel [H1_1 H1_2]].
+              rewrite H1_1 in H12. eapply Hrel in H12 as [k D].
+              eexists. constructor. reflexivity. simpl.
+              do 2 constructor. now apply Vrel_closed_r in H0.
+              do 2 constructor. congruence. rewrite vclosed_ignores_sub.
+              2: now apply Vrel_closed_r in H7.
+              rewrite map_map.
+              replace (map (fun x : Val => (` x).[hd'/]) tl') with
+                      (map VVal tl').
+              2: {
+                clear -H9. simpl.
+                apply biforall_vrel_closed in H9 as [_ H1].
+                apply map_ext_Forall. induction tl'; inv H1; constructor; auto.
+                now rewrite vclosed_ignores_sub.
+              }
+              constructor. now apply Vrel_closed_r in H7.
+              eapply step_term_term_plus. apply params_eval_create.
+              now apply biforall_vrel_closed in H9. simpl app. rewrite H1_2.
+              exact D. lia. eapply Frel_downclosed. eassumption.
+              Unshelve. lia. lia.
+            + repeat destruct_hyps.
+              rewrite H11 in H12. eapply H5 in H12 as [k D].
+              eexists. constructor. reflexivity. simpl.
+              do 2 constructor. now apply Vrel_closed_r in H0.
+              do 2 constructor. congruence. rewrite vclosed_ignores_sub.
+              2: now apply Vrel_closed_r in H7.
+              rewrite map_map.
+              replace (map (fun x : Val => (` x).[hd'/]) tl') with
+                      (map VVal tl').
+              2: {
+                clear -H9. simpl.
+                apply biforall_vrel_closed in H9 as [_ H1].
+                apply map_ext_Forall. induction tl'; inv H1; constructor; auto.
+                now rewrite vclosed_ignores_sub.
+              }
+              constructor. now apply Vrel_closed_r in H7.
+              eapply step_term_term_plus. apply params_eval_create.
+              now apply biforall_vrel_closed in H9. simpl app. rewrite H13.
+              exact D. simpl in Hmn1. lia.
+              eapply biforall_impl. 2: eassumption.
+              intros. downclose_Vrel.
+              Unshelve. lia.
+            + repeat destruct_hyps.
+              rewrite H11 in H12. eapply H5 in H12 as [k D].
+              eexists. constructor. reflexivity. simpl.
+              do 2 constructor. now apply Vrel_closed_r in H0.
+              do 2 constructor. congruence. rewrite vclosed_ignores_sub.
+              2: now apply Vrel_closed_r in H7.
+              rewrite map_map.
+              replace (map (fun x : Val => (` x).[hd'/]) tl') with
+                      (map VVal tl').
+              2: {
+                clear -H9. simpl.
+                apply biforall_vrel_closed in H9 as [_ H1].
+                apply map_ext_Forall. induction tl'; inv H1; constructor; auto.
+                now rewrite vclosed_ignores_sub.
+              }
+              constructor. now apply Vrel_closed_r in H7.
+              eapply step_term_term_plus. apply params_eval_create.
+              now apply biforall_vrel_closed in H9. simpl app. rewrite H13.
+              exact D. simpl in Hmn1. lia.
+              eapply Excrel_downclosed. eassumption.
+              Unshelve. simpl in Hmn1. lia.
+            + lia.
+            + lia.
+        * inv H8. (* Having 0 params in `catch` is exploited here,
+                     because we only want to evaluate the `of` subexpression
+                     in this `try` expression.
+                   *)
+          specialize (H12 _ _ _ _ eq_refl). contradiction.
+        * inv H7.
+      }
+
+      (* Finally, we combine the previous assertions with the closures
+         being in Rrel (H2). *)
+      inv Heval_e.
+      epose proof (H2 := H2 _ _ _ _ Hrel H11).
+      Unshelve. 2: lia.
+      clear -H2 H1. (* DANGER, nothing else is needed for now, however this
+                               is fragile if refactoring is needed *)
+      (* We deconstruct the evaluation in the premise: *)
+      inv H2. deriv. simpl in H9. deriv. deriv. simpl in H3.
+      deriv.
+      rewrite map_map in H6.
+      replace (map (fun x : Val => (` x).[VClos ext0 id0 (Datatypes.length vl1) e0/]) vl2) with
+                      (map VVal vl2) in H6.
+      2: {
+        clear -H1. simpl.
+        apply biforall_vrel_closed in H1 as [_ H1].
+        apply map_ext_Forall. induction vl2; inv H1; constructor; auto.
+        now rewrite vclosed_ignores_sub.
+      }
+      destruct vl2.
+      - deriv. simpl in H9. apply biforall_length in H1. rewrite H1 in H9.
+        simpl in H9. eexists. eassumption.
+      - deriv. deriv.
+        eapply term_step_term in H4. 2: apply params_eval_create.
+        2: {
+          apply biforall_vrel_closed in H1 as [_ H1]. now inv H1.
+        }
+        simpl in H4. apply biforall_length in H1. rewrite H1 in H4.
+        simpl in H4. rewrite Nat.eqb_refl in H4. eexists. eassumption.
+Qed.
+
+
+
+
+
+
+
+
+
+
+
+(* Lemma Rrel_Val_compat_closed_reverse :
+  forall (v v' : Val), forall m, Rrel m (`v) (`v') -> Vrel m v v'.
+Proof.
+  intros. apply CIU_Val_compat_closed_reverse.
+Qed.*)
+
+Corollary CIU_Val_compat_reverse :
+  forall Γ (v v' : Val), CIU_open Γ (`v) (`v') -> Vrel_open Γ v v'.
+Proof.
+  intros. unfold Vrel_open; intros.
+  epose proof (CIU_Val_compat_closed_reverse (v.[ξ₁]ᵥ) (v'.[ξ₁]ᵥ) ltac:(apply H) n).
+  epose proof (CIU_Val_compat_closed_reverse (v.[ξ₂]ᵥ) (v'.[ξ₂]ᵥ) ltac:(apply H) n).
+  Search Vrel subst.
+
+Qed.
+
+
 Lemma Erel_Val_compat_reverse :
   forall Γ (v v' : Val), Erel_open Γ (`v) (`v') -> Vrel_open Γ v v'.
 Proof.
@@ -1175,4 +1950,4 @@ Proof.
   apply H in H0. simpl in H0. destruct H0 as [HCl1 [HCl2 H0]].
   rewrite Vrel_Fix_eq. inv HCl1. inv HCl2.
   
-Qed.
+Qed. *)
